progress in sound_step of init analysis

rustfrontend/InitAnalysis.v
@@ -13,7 +13,7 @@ Local Open Scope list_scope.
 
 Definition moved_place (e: expr) : option place :=
   match e with
-  | Emoveplace p _ => Some p
+  | Emoveplace p _ => Some (valid_owner p)
   | _ => None
   end.
 
@@ -29,8 +29,10 @@ Fixpoint moved_place_list (al: list expr) : list place :=
 
 (* S is the whole set, flag = true indicates that it computes the MaybeInit set *)
 Definition transfer (S: PathsMap.t) (flag: bool) (f: function) (cfg: rustcfg) (pc: node) (before: PathsMap.t) : PathsMap.t :=
-  if PathsMap.beq before PathsMap.bot then PathsMap.bot
-  else
+  (* This condition complicates the proof. Maybe we can prove that
+  transfer bot = bot *)
+  (* if PathsMap.beq before PathsMap.bot then PathsMap.bot *)
+  (* else *)
     match cfg ! pc with
     | None => PathsMap.bot
     | Some (Inop _) => before
@@ -72,7 +74,7 @@ Local Open Scope error_monad_scope.
 
 (* The analyze returns the MaybeInit and MaybeUninit sets along with
 the universe set *)
-Definition analyze (ce: composite_env) (f: function) : Errors.res (PTree.t PathsMap.t * PTree.t PathsMap.t * PathsMap.t) :=
+Definition analyze (ce: composite_env) (f: function) : Errors.res (PMap.t PathsMap.t * PMap.t PathsMap.t * PathsMap.t) :=
   (* collect the whole set in order to simplify the gen and kill operation *)
   do whole <- collect_func ce f;
   (* initialize maybeInit set with parameters *)
@@ -87,11 +89,10 @@ Definition analyze (ce: composite_env) (f: function) : Errors.res (PTree.t Paths
   (* generate selector-based CFG for analysis *)
   do (entry, cfg) <- generate_cfg f.(fn_body);
   let initMap := DS.fixpoint cfg successors_instr (transfer whole true f cfg) entry maybeInit in
-let uninitMap := DS.fixpoint cfg successors_instr (transfer whole false f cfg) entry maybeUninit in
+  let uninitMap := DS.fixpoint cfg successors_instr (transfer whole false f cfg) entry maybeUninit in
   match initMap, uninitMap with
-  (* we only want the PTree because [None] represent the unreachable
-  node *)
-  | Some (_, initMap), Some (_, uninitMap) => Errors.OK (initMap, uninitMap, whole)
+  (* we only want the PTree because [None] represent the unreachable node *)
+  | Some initMap, Some uninitMap => Errors.OK (initMap, uninitMap, whole)
   | _, _ => Errors.Error (msg "Error in initialize analysis")
   end.
   
@@ -130,7 +131,7 @@ Definition must_movable (initmap uninitmap universemap: PathsMap.t) (p: place) :
     (Paths.filter (is_prefix p) universe).
 
 
-(** * Soundness of Initialized Analysis *)
+(** * Soundness of Initial Analysis *)
 
 
 (* relation between the selector and the (stmt, cont) pair *)
@@ -154,10 +155,14 @@ Inductive match_instr_stmt (body: statement) : instruction -> statement -> cont 
     match_instr_stmt body (Inop n) Scontinue k
 .
 
-(* Record sound_own (own: own_env) (init uninit: PathsMap.t) : Type := *)
-(*   PathsMap.t *)
-(*     Paths.diff *)
+Record sound_own (own: own_env) (init uninit universe: PathsMap.t) : Type :=
+  { sound_own_init: PathsMap.ge init own.(own_init);
+    
+    sound_own_uninit: PathsMap.ge uninit own.(own_uninit);
 
+    sound_own_universe: PathsMap.eq universe own.(own_universe) }.
+
+    
 (** ** Semantic invariant *)
 
 Section SOUNDNESS.
@@ -168,15 +173,146 @@ Variable se: Genv.symtbl.
 Let ge := RustIR.globalenv se prog.
 Let ce := ge.(genv_cenv).
 
-(* Inductive sound_state: state -> Prop := *)
-(* | sound_regular_state: forall *)
-(*     (AN: analyze ce f = OK (initMap, uninitMap)) *)
-(*     (INIT: initMap ! pc = Some mayinit) *)
-(*     (UNINIT: uninitMap ! pc = Some mayuninit) *)
-(*     (CFG: generate_cfg f.(fn_body) = OK (entry, cfg)) *)
-(*     (SEL: cfg ! pc = Some instr) *)
-(*     (IS: match_instr_stmt f.(fn_body) instr s k) *)
-(*     (OWN: sound_own own mayinit mayuninit) *)
-(*     sound_state (State f s k le own m) *)
+Inductive sound_cont: cont -> Prop :=
+| sound_cont_stop: sound_cont Kstop
+| sound_cont_seq: forall s k,
+    sound_cont k ->
+    sound_cont (Kseq s k)
+| sound_cont_loop: forall s k,
+    sound_cont k ->
+    sound_cont (Kloop s k)
+| sound_cont_call: forall f initMap uninitMap pc mayinit mayuninit universe entry cfg instr k own le p
+    (AN: analyze ce f = OK (initMap, uninitMap, universe))
+    (INIT: initMap !! pc = mayinit)
+    (UNINIT: uninitMap !! pc =  mayuninit)
+    (CFG: generate_cfg f.(fn_body) = OK (entry, cfg))
+    (SEL: cfg ! pc = Some instr)
+    (IS: match_instr_stmt f.(fn_body) instr Sskip k)
+    (OWN: sound_own own mayinit mayuninit universe)
+    (CONT: sound_cont k),
+    sound_cont (Kcall p f le own k)
+| sound_cont_dropplace: forall f initMap uninitMap pc mayinit mayuninit universe entry cfg instr k own le st l
+    (AN: analyze ce f = OK (initMap, uninitMap, universe))
+    (INIT: initMap !! pc =  mayinit)
+    (UNINIT: uninitMap !! pc =  mayuninit)
+    (CFG: generate_cfg f.(fn_body) = OK (entry, cfg))
+    (SEL: cfg ! pc = Some instr)
+    (IS: match_instr_stmt f.(fn_body) instr Sskip k)
+    (OWN: sound_own own mayinit mayuninit universe)
+    (CONT: sound_cont k),
+    sound_cont (Kdropplace f st l le own k)
+| sound_cont_dropcall: forall id b ofs st membs k,
+    sound_cont k ->
+    sound_cont (Kdropcall id (Vptr b ofs) st membs k)
+  .
+    
+Inductive sound_state: state -> Prop :=
+| sound_regular_state: forall f initMap uninitMap pc mayinit mayuninit universe entry cfg instr s k own le m
+    (AN: analyze ce f = OK (initMap, uninitMap, universe))
+    (INIT: initMap !! pc = mayinit)
+    (UNINIT: uninitMap !! pc = mayuninit)
+    (CFG: generate_cfg f.(fn_body) = OK (entry, cfg))
+    (SEL: cfg ! pc = Some instr)
+    (IS: match_instr_stmt f.(fn_body) instr s k)
+    (OWN: sound_own own mayinit mayuninit universe),
+    sound_state (State f s k le own m)
+| sound_callstate: forall vf args k m
+    (CONT: sound_cont k),
+    sound_state (Callstate vf args k m) 
+| sound_returnstate: forall v k m
+    (CONT: sound_cont k),
+    sound_state (Returnstate v k m)
+| sound_dropplace: forall f initMap uninitMap pc mayinit mayuninit universe entry cfg instr k own le st l m
+    (AN: analyze ce f = OK (initMap, uninitMap, universe))
+    (INIT: initMap !! pc = mayinit)
+    (UNINIT: uninitMap !! pc = mayuninit)
+    (CFG: generate_cfg f.(fn_body) = OK (entry, cfg))
+    (SEL: cfg ! pc = Some instr)
+    (IS: match_instr_stmt f.(fn_body) instr Sskip k)
+    (OWN: sound_own own mayinit mayuninit universe)
+    (CONT: sound_cont k),
+    sound_state (Dropplace f st l k le own m)
+| sound_dropstate: forall id b ofs st membs k m,
+    sound_cont k ->
+    sound_state (Dropstate id (Vptr b ofs) st membs k m)
+.
 
+(* use fixpoint_soulution to prove that the final abstract env
+approximates more than the abstract env computed by transfer
+function *)
+Lemma analyze_successor: forall f initMap uninitMap mayinit1 mayinit2 mayuninit1 mayuninit2 universe entry cfg instr pc1 pc2
+    (AN: analyze ce f = OK (initMap, uninitMap, universe))
+    (INIT: initMap !! pc1 = mayinit1)
+    (UNINIT: uninitMap !! pc1 = mayuninit1)
+    (CFG: generate_cfg f.(fn_body) = OK (entry, cfg))
+    (SEL: cfg ! pc1 = Some instr)
+    (PC: In pc2 (successors_instr instr))
+    (TFINIT: transfer universe true f cfg pc1 mayinit1 = mayinit2)
+    (TFUNINIT: transfer universe false f cfg pc1 mayuninit1 = mayuninit2),
+    PathsMap.ge (initMap !! pc2) mayinit1
+    /\ PathsMap.ge (uninitMap !! pc2) mayuninit1
+.
+  (* use fixpoint_solution *)
+Admitted.
+
+         
+(* use transfer to act as the bridge to construct the succ abstract
+env *)
+Lemma analyze_succ: forall f initMap uninitMap mayinit1 mayinit2 mayuninit1 mayuninit2 universe entry cfg instr own2 pc1 pc2
+    (AN: analyze ce f = OK (initMap, uninitMap, universe))
+    (INIT: initMap !! pc1 = mayinit1)
+    (UNINIT: uninitMap !! pc1 = mayuninit1)
+    (CFG: generate_cfg f.(fn_body) = OK (entry, cfg))
+    (SEL: cfg ! pc1 = Some instr)
+    (PC: In pc2 (successors_instr instr))
+    (TFINIT: transfer universe true f cfg pc1 mayinit1 = mayinit2)
+    (TFUNINIT: transfer universe false f cfg pc1 mayuninit1 = mayuninit2)
+    (OWN: sound_own own2 mayinit2 mayuninit2 universe),
+  exists mayinit3 mayuninit3,
+    initMap !! pc2 = mayinit3
+    /\ uninitMap !! pc2 = mayuninit3
+    /\ sound_own own2 mayinit3 mayuninit3 universe.
+  (* show that PathsMap.ge ae1 ae2 and sound_own ae1 implies sound_own
+  ae2 *)
+Admitted.
+
+Lemma sound_state_succ: forall f initMap uninitMap mayinit1 mayinit2 mayuninit1 mayuninit2 universe entry cfg instr1 instr2 own2 pc1 pc2 s k m le
+    (AN: analyze ce f = OK (initMap, uninitMap, universe))
+    (INIT: initMap !! pc1 = mayinit1)
+    (UNINIT: uninitMap !! pc1 = mayuninit1)
+    (CFG: generate_cfg f.(fn_body) = OK (entry, cfg))
+    (SEL1: cfg ! pc1 = Some instr1)
+    (PC: In pc2 (successors_instr instr1))
+    (* how to prove it? *)
+    (SEL2: cfg ! pc2 = Some instr2)
+    (IS: match_instr_stmt f.(fn_body) instr2 s k)
+    (TFINIT: transfer universe true f cfg pc1 mayinit1 = mayinit2)
+    (TFUNINIT: transfer universe false f cfg pc1 mayuninit1 = mayuninit2)
+    (OWN: sound_own own2 mayinit2 mayuninit2 universe),
+    sound_state (State f s k le own2 m).
+Admitted.
+
+
+Theorem sound_step: forall s t s',
+    step ge s t s' ->
+    sound_state s ->
+    sound_state s'.
+Proof.
+  intros s t s' STEP SOUND.
+  inv STEP; inv SOUND.
+  (* step_assign *)
+  - inv IS.
+    eapply sound_state_succ with (pc2:= n); eauto.
+    simpl. auto.
+    (* TODO: properties of generated cfg *)
+    admit.
+    admit.
+    (* prove sound_own *)
+    inv OWN.
+    unfold transfer. rewrite SEL. rewrite H3.
+    (* maybe easy *)
+    unfold own_check_expr, own_check_assign in *.
+    admit.
+Admitted.      
+    
 End SOUNDNESS.
